src/StVM.v
@@ -4,15 +4,13 @@ Record representing the AVM Monad state structure.
 Author:  Adam Petz, ampetz@ku.edu
 *)
 
-Require Import MyStack ConcreteEvidence.
+Require Import ConcreteEvidence.
 Require Import Maps.
 
 (* Specific VM monad state *)
-Definition ev_stack := gen_stack EvidenceC.
 Definition ev_store := Map.
 Record vm_st : Type := mk_st
                          {st_ev:EvidenceC ;
-                          st_stack:ev_stack ; 
                           st_trace:list Ev ;
                           st_pl:Plc ;
                           st_store:ev_store}.
